02Stack/StackCorrectness.thy
@@ -2,9 +2,9 @@ theory StackCorrectness
 imports StackConversion "../01Expression/Evaluate" "../Utilities/Iterate"
 begin
 
-lemma complete': "unstack_state rs \<Sigma> \<leadsto> e' \<Longrightarrow> \<exists>\<Sigma>'. \<Sigma> \<leadsto>\<^sub>s \<Sigma>' \<and> unstack_state rs \<Sigma>' = e'"
-  proof (induction "unstack_state rs \<Sigma>" e' rule: evaluate.induct) 
-  case ev_app1
+lemma complete': "e \<leadsto> e' \<Longrightarrow> unstack_state rs \<Sigma> = e \<Longrightarrow> \<exists>\<Sigma>'. \<Sigma> \<leadsto>\<^sub>s \<Sigma>' \<and> unstack_state rs \<Sigma>' = e'"
+  proof (induction e e' rule: evaluate.induct) 
+  case (ev_app1 e\<^sub>1 e\<^sub>1' e\<^sub>2)
     thus ?case by simp 
   next case ev_app2 
     thus ?case by simp 
@@ -44,7 +44,7 @@ lemma complete': "unstack_state rs \<Sigma> \<leadsto> e' \<Longrightarrow> \<ex
     thus ?case by simp 
   qed 
 
-lemma complete: "iter (op \<leadsto>) e e' \<Longrightarrow> unstack_state \<Sigma> e \<Longrightarrow>
+lemma complete: "iter (op \<leadsto>) e e' \<Longrightarrow> unstack_state rs \<Sigma> e \<Longrightarrow>
     \<exists>\<Sigma>'. iter (op \<leadsto>\<^sub>s) \<Sigma> \<Sigma>' \<and> unstack_state \<Sigma>' e'"
   proof (induction e e' arbitrary: \<Sigma> rule: iter.induct)
   case iter_refl
